end2end: wip fixing [pc_related]

processor/src/processor/FetchOk.v
@@ -20,6 +20,13 @@ Require Import processor.KamiProc.
 
 Local Open Scope Z_scope.
 
+Lemma wordToN_eq_rect:
+  forall sz (w: Word.word sz) nsz Hsz,
+    wordToN (eq_rect _ Word.word w nsz Hsz) = wordToN w.
+Proof.
+  intros; subst; simpl; reflexivity.
+Qed.
+
 Lemma Z_pow_add_lor:
   forall n m p: Z,
     0 <= n < 2 ^ p -> 0 <= m -> 0 <= p ->
@@ -143,42 +150,46 @@ Section FetchOk.
 
   Definition pc_related (kpc: Word.word (2 + Z.to_nat instrMemSizeLg))
              (rpc: kword width): Prop :=
-    #kpc = #rpc.
+    wordToN kpc = wordToN rpc.
 
   Definition AddrAligned (addr: kword width) :=
     split1 2 (nwidth - 2) addr = WO~0~0.
 
-  Definition makeAlignedXAddr (base: kword (width - 2)) (n: nat): word :=
+  Definition alignedXAddr (base: kword (width - 2)) (n: nat): word :=
     Word.combine WO~0~0 (base ^+ natToWord (nwidth - 2)%nat n).
 
-  Fixpoint makeAlignedXAddrs (base: kword (width - 2)) (n: nat): XAddrs :=
+  Definition alignedXAddrs (base: kword (width - 2)) (n: nat): XAddrs :=
+    [alignedXAddr base n; alignedXAddr base n ^+ $1;
+       alignedXAddr base n ^+ $2; alignedXAddr base n ^+ $3].
+
+  Fixpoint alignedXAddrsRange (base: kword (width - 2)) (n: nat): XAddrs :=
     match n with
     | O => nil
-    | S n' => makeAlignedXAddr base n :: makeAlignedXAddrs base n'
+    | S n' => alignedXAddrs base n' ++ alignedXAddrsRange base n'
     end.
 
-  Lemma makeAlignedXAddrs_AddrAligned:
-    forall base n x,
-      In x (makeAlignedXAddrs base n) ->
-      AddrAligned x.
-  Proof.
-    induction n; intros; [exfalso; auto|].
-    destruct H.
-    - subst; reflexivity.
-    - auto.
-  Qed.
+  (* Lemma makeAlignedXAddrs_AddrAligned: *)
+  (*   forall base n x, *)
+  (*     In x (makeAlignedXAddrs base n) -> *)
+  (*     AddrAligned x. *)
+  (* Proof. *)
+  (*   induction n; intros; [exfalso; auto|]. *)
+  (*   destruct H. *)
+  (*   - subst; reflexivity. *)
+  (*   - auto. *)
+  (* Qed. *)
 
   (* set of executable addresses in the kami processor *)
   Definition kamiXAddrs: XAddrs :=
     (* addXAddrRange (wzero _) instrMemSize nil. *)
-    makeAlignedXAddrs (wzero _) instrMemSize.
+    alignedXAddrsRange (wzero _) instrMemSize.
 
-  Corollary kamiXAddrs_In_AddrAligned:
-    forall addr, In addr kamiXAddrs -> AddrAligned addr.
-  Proof.
-    intros.
-    eapply makeAlignedXAddrs_AddrAligned; eassumption.
-  Qed.
+  (* Corollary kamiXAddrs_In_AddrAligned: *)
+  (*   forall addr, In addr kamiXAddrs -> AddrAligned addr. *)
+  (* Proof. *)
+  (*   intros. *)
+  (*   eapply makeAlignedXAddrs_AddrAligned; eassumption. *)
+  (* Qed. *)
 
   Lemma pc_related_preserves_AddrAligned:
     forall kpc rpc,
@@ -199,16 +210,17 @@ Section FetchOk.
     remember (split2 2 (nwidth - 2) rpc) as rpcr; clear Heqrpcr.
     clear H1 rpc; subst rpcl.
 
-    rewrite wordToNat_combine in H.
+    rewrite wordToN_combine in H.
     change (Z.to_nat width) with (2 + (nwidth - 2))%nat in H.
-    rewrite wordToNat_combine in H.
+    rewrite wordToN_combine in H.
 
-    change (NatLib.pow2 2) with 4%nat in H.
-    do 2 rewrite Nat.mul_comm with (n:= 4%nat) in H.
-    apply f_equal with (f:= fun x => Nat.modulo x 4%nat) in H.
-    do 2 rewrite Nat.mod_add in H by discriminate.
-    do 2 rewrite Nat.mod_small in H by apply wordToNat_bound.
-    apply wordToNat_inj; assumption.
+    change (NatLib.Npow2 2) with 4%N in H.
+    do 2 rewrite N.mul_comm with (n:= 4%N) in H.
+    
+    apply f_equal with (f:= fun x => N.modulo x 4%N) in H.
+    do 2 rewrite N.mod_add in H by discriminate.
+    do 2 rewrite N.mod_small in H by apply wordToN_bound.
+    apply wordToN_inj; assumption.
   Qed.
 
   Definition mem_related (kmem: kword width -> kword 8)
@@ -222,14 +234,16 @@ Section FetchOk.
              (xaddrs: XAddrs) :=
     forall rpc,
       isXAddr4 rpc xaddrs ->
-      AddrAligned rpc /\
-      (forall kpc, pc_related kpc rpc ->
-                   Kami.Ex.SC.combineBytes 4%nat rpc kmemd =
-                   kmemi (split2 2 _ kpc)).
+      isXAddr4 rpc kamiXAddrs /\
+      (AddrAligned rpc ->
+       forall kpc,
+         pc_related kpc rpc ->
+         Kami.Ex.SC.combineBytes 4%nat rpc kmemd =
+         kmemi (split2 2 _ kpc)).
 
   Lemma rv32AlignAddr_consistent:
     forall rpc kpc,
-      In rpc kamiXAddrs ->
+      AddrAligned rpc ->
       pc_related kpc rpc ->
       evalExpr
         (IsaRv32.rv32AlignAddr
@@ -243,20 +257,19 @@ Section FetchOk.
     cbv [evalExpr evalBinBit evalUniBit].
     cbv [evalConstT].
 
-    apply wordToNat_inj.
-    rewrite wordToNat_eq_rect.
-    do 2 rewrite wordToNat_combine.
+    apply wordToN_inj.
+    rewrite wordToN_eq_rect.
+    do 2 rewrite wordToN_combine.
     do 2 rewrite ZToWord_zero.
-    do 2 rewrite wordToNat_wzero.
-    rewrite Nat.mul_0_r, Nat.add_0_r, Nat.add_0_l.
+    do 2 rewrite wordToN_wzero.
+    rewrite N.mul_0_r, N.add_0_r, N.add_0_l.
 
     rewrite <-H0.
     rewrite <-(Word.combine_split 2 ninstrMemSizeLg kpc) at 2.
 
-    apply kamiXAddrs_In_AddrAligned in H.
     pose proof (pc_related_preserves_AddrAligned _ _ H0 H).
     rewrite H1.
-    rewrite wordToNat_combine.
+    rewrite wordToN_combine.
     reflexivity.
   Qed.
 
@@ -307,6 +320,7 @@ Section FetchOk.
            (rmemd: mem)
            (rpc: kword width),
       isXAddr4 rpc xaddrs ->
+      AddrAligned rpc ->
       pc_related kpc rpc ->
       mem_related kmemd rmemd ->
       exists (rinst: HList.tuple byte 4),
@@ -315,8 +329,8 @@ Section FetchOk.
   Proof.
     intros.
     specialize (Hxs _ H); destruct Hxs.
-    specialize (H3 _ H0).
-    rewrite <-H3.
+    specialize (H4 H0 _ H1).
+    rewrite <-H4.
     eapply getmany_of_tuple_combineBytes_consistent.
     assumption.
   Qed.
